\documentclass{article}
\usepackage{epsfig}
\pagestyle{empty}
\begin{document}
$\sigma$
\pagebreak

$ (pre.x-post.x)^2/a^2 + (pre.y-post.y)/b^2 <= 1 $
\pagebreak

$pre.z==post.z$
\pagebreak

$ (pre.x-post.x)^2/a^2 + (pre.y-post.y)/b^2 == 1$
\pagebreak

$ pre.x = pre.x / gridPre.x * gridPost.x $
\pagebreak

$ pre.y = pre.y / gridPre.y * gridPost.y $
\pagebreak

$ pre.z = pre.z / gridPre.z * gridPost.z $
\pagebreak

$i_{10}$
\pagebreak

\begin{align*} i_{10} = & G_0^{down} (v_{10} - v_{0}) + G_5^{down} (v_{10} - v_{5}) + G_{15}^{up} (v_{10} - v_{15}), & \text{(1)} \end{align*}
\pagebreak

$v_n$
\pagebreak

$G_n^{down}$
\pagebreak

$G_n^{up}$
\pagebreak

\end{document}
